Initial work on proving reverseSlice

go/iterator/iter_test.go
@@ -1,6 +1,7 @@
 package iterator
 
 import (
+	"reflect"
 	"testing"
 )
 
@@ -31,5 +32,20 @@ func TestIsAsciiTrue(t *testing.T) {
 func TestIsAsciiFalse(t *testing.T) {
 	if isAscii([]byte("∃non∧sciiCharInthisString")) {
 		t.Errorf(`"∃non∧sciiCharInthisString" is not an ASCII string!`)
+	}
+}
+
+func TestReverseSliceEmpty(t *testing.T) {
+	if !reflect.DeepEqual([]int{}, reverseSlice([]int{})) {
+		t.Errorf(`[] is the reverse of itself!`)
+	}
+}
+
+func TestReverseSlice0(t *testing.T) {
+	s := []int{1, 2, 3, 4, 5, 6, 7}
+	rev_s := []int{7, 6, 5, 4, 3, 2, 1}
+
+	if !reflect.DeepEqual(rev_s, reverseSlice(s)) {
+		t.Errorf(`[7 ... 0] was not reversed correctly!`)
 	}
 }
